thy/Bitmagic/Numberwang_Ln.thy
@@ -1,5 +1,5 @@
 theory Numberwang_Ln
-imports NumberWangCebewee NumberWangCaesar IPv4Addr
+imports NumberWangCebewee PrefixMatch IPv4Addr
 begin
 
 (*TODO: move to IpAddresses or somewhere*)
