thy/Primitive_Matchers/IpAddresses.thy
@@ -58,8 +58,6 @@ by(simp add: ipv4addr_of_dotdecimal.simps ipv4addr_of_nat_def ipv4range_set_from
         Some (base2, m2)
       )"
 
-
-
   (*TODO: move*)
   lemma ipcidr_conjunct_any: "ipcidr_conjunct (0, 0) (0, 0) \<noteq> None"
     by(simp add: ipset_from_cidr_0)
